induction principles for validity

theories/Validity.v
@@ -164,7 +164,7 @@ Section MoreDefs.
 
   Definition validEmpty : [||-v ε ] := Build_VAdequate emptyVPack VREmpty.
 
-  Definition validSnoc {Γ na A l} (VΓ : [||-v Γ]) (VA : [Γ ||-v< l > A | VΓ]) 
+  Definition validSnoc {Γ} na {A l} (VΓ : [||-v Γ]) (VA : [Γ ||-v< l > A | VΓ]) 
     : [||-v Γ ,, vass na A ] :=
     Build_VAdequate (snocVPack Γ VΓ A l VA na) (VRSnoc VΓ VΓ VA).
 
@@ -225,3 +225,31 @@ Notation "[ Γ ||-v< l > t : A | VΓ | VA ]"     := (termValidity Γ l t A VΓ V
 Notation "[ Γ ||-v< l > A ≅ B | VΓ | VA ]"     := (typeEqValidity Γ l A B VΓ VA) (at level 0, Γ, l, A, B, VΓ, VA at level 50).
 Notation "[ Γ ||-v< l > t ≅ u : A | VΓ | VA ]" := (termEqValidity Γ l t u A VΓ VA) (at level 0, Γ, l, t, u, A, VΓ, VA at level 50).
 Notation "[ Γ ||-v< l > t ≅ u : A | VΓ ]"      := (tmEqValidity Γ l t u A VΓ) (at level 0, Γ, l, t, u, A, VΓ at level 50).
+
+Section Inductions.
+  Context `{ta : tag} `{WfContext ta} `{WfType ta} `{Typing ta}
+  `{ConvType ta} `{ConvTerm ta} `{ConvNeu ta} `{RedType ta} `{RedTerm ta}.
+  
+  Theorem VR_rect
+    (P : forall {Γ vSubst vSubstExt}, VR Γ vSubst vSubstExt -> Type) 
+    (hε : P VREmpty)
+    (hsnoc : forall {Γ na A l VΓ VΓad VA}, 
+      P VΓad -> P (VRSnoc (Γ := Γ) (na := na) (A := A) (l := l) VΓ VΓad VA)) :
+    forall {Γ vSubst vSubstExt} (VΓ : VR Γ vSubst vSubstExt), P VΓ.
+  Proof.
+    fix ih 4; destruct VΓ; [exact hε | apply hsnoc; apply ih].
+  Defined.
+  
+  Theorem validity_rect
+    (P : forall {Γ : context}, [||-v Γ] -> Type)
+    (hε : P validEmpty)
+    (hsnoc : forall {Γ na A l} (VΓ : [||-v Γ]) (VA : [Γ ||-v< l > A | VΓ]), P VΓ -> P (validSnoc na VΓ VA)) :
+    forall {Γ : context} (VΓ : [||-v Γ]), P VΓ.
+  Proof.
+    intros Γ [[s eq] VΓad]; revert Γ s eq VΓad.
+    apply VR_rect.
+    - apply hε.
+    - intros *; apply hsnoc.
+  Defined.
+  
+End Inductions.
